changes to allow using different input buffers for the same flight

src/tls/HSL.Receive.fst
@@ -16,39 +16,31 @@ open HSL.Common
 
 #reset-options "--max_fuel 0 --max_ifuel 0 --using_facts_from '* -FStar.Tactics -FStar.Reflection'"
 
+type inc_st_t = G.erased (bytes & in_progress_flt_t)
+
 noeq
 type hsl_state = {
   rgn: Mem.rgn;
-  from_to: B.pointer (option range_t);
-  parsed_bytes: (p:B.pointer (G.erased bytes){
-   let open B in
-   let locs =
-     [loc_buffer from_to;
-      loc_buffer p]
-   in
-    all_disjoint locs /\
-    rgn `region_includes` B.loc_union_l locs
+  inc_st: (p:B.pointer inc_st_t{
+    rgn `region_includes` B.loc_buffer p
   });
 }
 
-let region_of s = s.rgn
+let region_of st = st.rgn
 
-let index_from_to s h = B.deref h s.from_to
+let parsed_bytes st h = fst (G.reveal (B.deref h st.inc_st))
 
-let parsed_bytes s h = G.reveal (B.deref h s.parsed_bytes)
+let in_progress_flt st h = snd (G.reveal (B.deref h st.inc_st))
 
-let invariant s h =
-  B.live h s.from_to /\
-  B.live h s.parsed_bytes
+let invariant s h = B.live h s.inc_st
 
-let footprint s = B.(loc_union (loc_buffer s.from_to) (loc_buffer s.parsed_bytes))
+let footprint s = B.loc_buffer s.inc_st
 
 let frame_hsl_state _ _ _ _ = ()
 
 let create r =
-  let from_to = B.malloc r None 1ul in
-  let parsed_bytes = B.malloc r (G.hide (Seq.empty)) 1ul in
-  { rgn = r; from_to = from_to; parsed_bytes = parsed_bytes }
+  let inc_st = B.malloc r (G.hide (Seq.empty, F_none)) 1ul in
+  { rgn = r; inc_st = inc_st }
 
 let receive_flight13_ee_c_cv_fin _ _ _ _ = admit()
 let receive_flight13_ee_cr_c_cv_fin _ _ _ _ = admit ()
